src/Parsers/Refinement/DisjointRules.v
@@ -4,6 +4,8 @@ Require Import Fiat.Parsers.Refinement.Tactics.
 Require Import Fiat.Computation.Refinements.General.
 Require Import Fiat.Parsers.StringLike.Properties.
 Require Import Fiat.Parsers.StringLike.String.
+Require Import Fiat.Parsers.StringLike.FirstCharSuchThat.
+Require Import Fiat.Parsers.StringLike.FirstChar.
 Require Import Fiat.Common.
 Require Import Fiat.Common.Equality.
 Require Import Fiat.Common.List.Operations.
@@ -11,8 +13,167 @@ Require Import Fiat.Parsers.Splitters.RDPList.
 Require Import Fiat.Parsers.BaseTypes.
 Require Import Fiat.Parsers.Refinement.DisjointLemmas.
 Require Import Fiat.Parsers.ParserInterface.
+Require Import Fiat.Parsers.StringLike.Core.
 
 Set Implicit Arguments.
+
+Definition search_for_condition (G : grammar Ascii.ascii) str its (n : nat)
+  := is_first_char_such_that
+       (might_be_empty (possible_first_terminals_of_production G its))
+       str
+       n
+       (fun ch => list_bin ascii_beq ch (possible_first_terminals_of_production G its)).
+
+Lemma refine_disjoint_search_for' {G : grammar Ascii.ascii} {str nt its}
+      (H_disjoint : disjoint ascii_beq
+                             (possible_terminals_of G nt)
+                             (possible_first_terminals_of_production G its))
+: refine {splits : list nat
+         | split_list_is_complete
+             G str
+             (NonTerminal nt)
+             its splits}
+         (n <- { n : nat | n <= length str
+                           /\ ((exists n', search_for_condition G str its n')
+                               -> search_for_condition G str its n) };
+          ret [n]).
+Proof.
+  intros ls H.
+  computes_to_inv; subst.
+  destruct H as [H0 H1].
+  apply PickComputes.
+  intros n ? H_reachable pit pits Hpit Hpits.
+  left.
+  pose proof (terminals_disjoint_search_for _ H_disjoint _ _ H_reachable Hpit Hpits) as H'.
+  specialize (H1 (ex_intro _ n H')).
+  pose proof (is_first_char_such_that_eq_nat_iff H1 H') as H''.
+  destruct_head or; destruct_head and; subst; omega.
+Qed.
+
+Definition search_for_not_condition (G : grammar Ascii.ascii) str nt its n
+  := is_first_char_such_that
+       (might_be_empty (possible_first_terminals_of_production G its))
+       str
+       n
+       (fun ch => negb (list_bin ascii_beq ch (possible_terminals_of G nt))).
+
+Lemma refine_disjoint_search_for_not' {G : grammar Ascii.ascii} {str nt its}
+      (H_disjoint : disjoint ascii_beq
+                             (possible_terminals_of G nt)
+                             (possible_first_terminals_of_production G its))
+: refine {splits : list nat
+         | split_list_is_complete
+             G str
+             (NonTerminal nt)
+             its splits}
+         (n <- { n : nat | n <= length str
+                           /\ ((exists n', search_for_not_condition G str nt its n')
+                               -> search_for_not_condition G str nt its n) };
+          ret [n]).
+Proof.
+  intros ls H.
+  computes_to_inv; subst.
+  destruct H as [H0 H1].
+  apply PickComputes.
+  intros n ? H_reachable pit pits Hpit Hpits.
+  left.
+  pose proof (terminals_disjoint_search_for_not _ H_disjoint _ _ H_reachable Hpit Hpits) as H'.
+  specialize (H1 (ex_intro _ n H')).
+  pose proof (is_first_char_such_that_eq_nat_iff H1 H') as H''.
+  destruct_head or; destruct_head and; subst; omega.
+Qed.
+
+Lemma find_first_char_such_that'_short {Char HSL}
+      str P len
+: @find_first_char_such_that' Char HSL P len str <= len.
+Proof.
+  revert str; induction len; simpl; intros; [ reflexivity | ].
+  destruct (get (length str - S len) str) eqn:H.
+  { edestruct P; try omega.
+    apply Le.le_n_S, IHlen. }
+  { apply Le.le_n_S, IHlen. }
+Qed.
+
+Lemma find_first_char_such_that_short {Char HSL}
+      str P
+: @find_first_char_such_that Char HSL str P <= length str.
+Proof.
+  apply find_first_char_such_that'_short.
+Qed.
+
+Lemma is_first_char_such_that__find_first_char_such_that {Char} {HSL} {HSLP : @StringLikeProperties Char HSL} str P
+      might_be_empty
+      (H : exists n, is_first_char_such_that might_be_empty str n (fun ch => is_true (P ch)))
+: is_first_char_such_that might_be_empty str (@find_first_char_such_that Char HSL str P) (fun ch => is_true (P ch)).
+Proof.
+  unfold find_first_char_such_that.
+  destruct H as [n H].
+  set (len := length str).
+  setoid_replace str with (drop (length str - len) str) at 1
+    by (subst; rewrite Minus.minus_diag, drop_0; reflexivity).
+  setoid_replace str with (drop (length str - len) str) in H
+    by (subst; rewrite Minus.minus_diag, drop_0; reflexivity).
+  assert (len <= length str) by reflexivity.
+  clearbody len.
+  generalize dependent str; revert n.
+  induction len; simpl; intros n str IH Hlen.
+  { apply first_char_such_that_0.
+    rewrite drop_length.
+    rewrite NPeano.Nat.sub_0_r in IH |- *.
+    rewrite Minus.minus_diag.
+    split.
+    { apply for_first_char_nil.
+      rewrite drop_length; omega. }
+    { generalize dependent str.
+      induction n; intros str H Hlen.
+      { apply first_char_such_that_0 in H.
+        rewrite drop_length, Minus.minus_diag in H.
+        destruct_head and; trivial. }
+      { apply first_char_such_that_past_end in H; [ | rewrite drop_length; omega ].
+        left; assumption. } } }
+  { pose proof (singleton_exists (take 1 (drop (length str - S len) str))) as H'.
+    rewrite take_length, drop_length in H'.
+    destruct H' as [ch H']; [ apply Min.min_case_strong; intros; omega | ].
+    rewrite get_drop.
+    rewrite (proj1 (get_0 _ _) H').
+    destruct (P ch) eqn:H''.
+    { apply first_char_such_that_0.
+      rewrite drop_length.
+      split; [ | right; omega ].
+      apply (for_first_char__take 0).
+      rewrite <- for_first_char_singleton by eassumption; trivial. }
+    { apply is_first_char_such_that_drop.
+      destruct n.
+      { apply first_char_such_that_0 in IH.
+        destruct IH as [IH _].
+        apply (for_first_char__take 0) in IH.
+        rewrite <- for_first_char_singleton in IH by eassumption; unfold is_true in *; congruence. }
+      { apply is_first_char_such_that_drop in IH.
+        destruct IH as [IH _].
+        rewrite drop_drop in IH |- *; simpl in IH |- *.
+        replace (S (length str - S len)) with (length str - len) in IH |- * by omega.
+        split.
+        { eapply IHlen; try eassumption; [].
+          omega. }
+        { apply (for_first_char__take 0).
+          rewrite <- for_first_char_singleton by eassumption; congruence. } } } }
+Qed.
+
+Lemma refine_find_first_char_such_that {Char} {HSL : StringLike Char} {HSLP : @StringLikeProperties Char HSL}
+      (str : @String Char HSL)
+      (P : Char -> bool)
+      might_be_empty
+: refine { n : nat | n <= length str
+                     /\ ((exists n', is_first_char_such_that might_be_empty str n' P)
+                         -> is_first_char_such_that might_be_empty str n P) }
+         (ret (find_first_char_such_that str P)).
+Proof.
+  intros v H.
+  computes_to_inv; subst.
+  apply PickComputes.
+  split; [ apply find_first_char_such_that_short | ].
+  apply is_first_char_such_that__find_first_char_such_that.
+Qed.
 
 Lemma refine_disjoint_search_for {G : grammar Ascii.ascii} {str nt its}
       (H_disjoint : disjoint ascii_beq
@@ -23,45 +184,25 @@ Lemma refine_disjoint_search_for {G : grammar Ascii.ascii} {str nt its}
              G str
              (NonTerminal nt)
              its splits}
-         (n <- { n : nat | n <= length str
-                           /\ is_first_char_such_that
-                                (might_be_empty (possible_first_terminals_of_production G its))
-                                str
-                                n
-                                (fun ch => list_bin ascii_beq ch (possible_first_terminals_of_production G its)) };
-          ret [n]).
+         (ret [find_first_char_such_that str (fun ch => list_bin ascii_beq ch (possible_first_terminals_of_production G its))]).
 Proof.
-  intros ls H.
-  computes_to_inv; subst.
-  destruct H as [H0 H1].
-  apply PickComputes.
-  intros n ? H_reachable pit pits Hpit Hpits.
-  left.
-  pose proof (terminals_disjoint_search_for _ H_disjoint _ _ H_reachable Hpit Hpits) as H'.
-  Locate disjoint.
+  rewrite refine_disjoint_search_for' by assumption.
+  setoid_rewrite refine_find_first_char_such_that.
+  simplify with monad laws; reflexivity.
+Qed.
 
-(first_char_in
-            (drop n str)
-            (possible_first_terminals_of_production G its)
-Lemma terminals_disjoint_search_for {G : grammar Ascii.ascii} (str : @String Ascii.ascii string_stringlike)
-      {nt its}
-      (H_disjoint : disjoint ascii_beq (possible_terminals_of G nt) (possible_first_terminals_of_production G its))
-      {n}
-      (pit : parse_of_item G (StringLike.take n str) (NonTerminal nt))
-      (pits : parse_of_production G (StringLike.drop n str) its)
-      (H_reachable : production_is_reachable G (NonTerminal nt :: its))
-      (Hpit : Forall_parse_of_item (fun _ nt => List.In nt (Valid_nonterminals G)) pit)
-      (Hpits : Forall_parse_of_production (fun _ nt => List.In nt (Valid_nonterminals G)) pits)
-: forall_chars (take n str)
-               (fun ch => negb (list_bin ascii_beq ch (possible_first_terminals_of_production G its)))
-  /\ ((length str <= n /\ might_be_empty (possible_first_terminals_of_production G its))
-      \/ (first_char_in
-            (drop n str)
-            (possible_first_terminals_of_production G its))).
+Lemma refine_disjoint_search_for_not {G : grammar Ascii.ascii} {str nt its}
+      (H_disjoint : disjoint ascii_beq
+                             (possible_terminals_of G nt)
+                             (possible_first_terminals_of_production G its))
+: refine {splits : list nat
+         | split_list_is_complete
+             G str
+             (NonTerminal nt)
+             its splits}
+         (ret [find_first_char_such_that str (fun ch => negb (list_bin ascii_beq ch (possible_terminals_of G nt)))]).
 Proof.
-
-{splits : list nat |
-                       ParserInterface.split_list_is_complete
-                         plus_expr_grammar (string_of_indexed r_n)
-                         (NonTerminal "number")
-                         [Terminal "+"%char; NonTerminal "expr"] splits}
+  rewrite refine_disjoint_search_for_not' by assumption.
+  setoid_rewrite refine_find_first_char_such_that.
+  simplify with monad laws; reflexivity.
+Qed.
